Create command line functionality -- Long
This commit contains an old proof in case the hd/tl functions
are changed to be more efficient

basis/mlcommandLineProgScript.sml
@@ -1,5 +1,5 @@
 open preamble
-     ml_translatorLib ml_progLib
+     ml_translatorLib ml_progLib miscTheory
      cfTheory cfHeapsTheory cfTacticsLib cfTacticsBaseLib basisFunctionsLib
      mlcharioProgTheory ml_progLib ml_translatorTheory
 
@@ -23,6 +23,23 @@ val w8arrayToStrings = process_topdecs
 val res = ml_prog_update (ml_progLib.add_prog w8arrayToStrings pick_name)
 
 val e =
+  ``LetApps "cs" (Long "Word8Array" "array") [Lit (IntLit 256); Lit (Word8 0w)] (
+      Let NONE (App (FFI "getArgs") [Var (Short "cs")])
+        (Apps [Var (Short "w8arrayToStrings"); Var (Short "cs")]))``
+  |> EVAL |> concl |> rand
+
+val _ = ml_prog_update(add_Dlet_Fun ``"cline"`` ``"u"`` e "cline_v")
+
+val name = process_topdecs `fun name u = List.hd (cline ())`
+
+val _ = ml_prog_update(ml_progLib.add_prog name pick_name)
+
+val arguments = process_topdecs `fun arguments u = List.tl (cline ())`
+      
+val _ = ml_prog_update(ml_progLib.add_prog arguments pick_name)
+
+(*
+val e =
   ``Let NONE (App (FFI "getArgs") [Var (Short "commandLine_state")])
       (LetApps "ss" (Short "w8arrayToStrings") [Var (Short "commandLine_state")]
         (Apps [Var (Long "List" "hd"); Var (Short "ss")]))``
@@ -37,7 +54,7 @@ val e =
   |> EVAL |> concl |> rand
 
 val _ = ml_prog_update(add_Dlet_Fun ``"arguments"`` ``"u"`` e "arguments_v")
-
+*)
 val _ = ml_prog_update (close_module NONE);
 
 
@@ -58,11 +75,17 @@ val commandLine_fun_def = Define `
         else NONE 
       | _ => NONE)`
 
+(*
 val COMMANDLINE_def = Define `
   COMMANDLINE (cl:string list) =
     IO (List (MAP Str cl)) commandLine_fun ["getArgs"] *
     SEP_EXISTS w. W8ARRAY commandLine_state w * &(LENGTH w = 256)` 
+*)
 
+val COMMANDLINE_def = Define `
+  COMMANDLINE (cl:string list) =
+    IO (List (MAP Str cl)) commandLine_fun ["getArgs"]`
+ 
 val st = get_ml_prog_state()
 (*
 options:
@@ -155,125 +178,255 @@ val w8arrayToStrings_spec = Q.store_thm ("w8arrayToStrings_spec",
 
 
 val map_app_last_thm = Q.prove(
-  `!ls a. ls <> [] ==> ?l. FLAT(MAP (\x. x ++ [a]) ls) = l ++ [a]`,
-  Induct \\ rw[] \\ first_x_assum(qspecl_then [`a`] mp_tac) \\ Cases_on `ls`
-  \\ rw[] \\ qexists_tac `h++[a]++l` \\ rw[] 
+  `!ls a. ls <> [] ==> (FLAT(MAP (\x. x ++ [a]) ls) = FLAT(MAP (\x. x ++ [a]) (BUTLAST ls)) ++ (LAST ls) ++ [a])`,
+  Induct \\ rw[] \\ first_x_assum(qspecl_then [`a`] mp_tac) \\ Cases_on `ls` \\ rw[]
 );
+
 
 val map_app_last_Str = Q.prove(
-  `!ls. ls <> [] ==> ?l.
-      CONCAT(MAP(\s. STRCAT (destStr s) "\^@") (MAP Str ls)) =  l ++ [CHR 0]`,
-  Induct \\ rw[] \\ Cases_on `ls` \\ rw[] \\ qexists_tac `h++[CHR 0]++l` \\ rw[]
+  `!ls. ls <> [] ==>
+      CONCAT(MAP(\s. STRCAT (destStr s) "\^@") (MAP Str ls)) = FRONT(CONCAT(MAP(\s. STRCAT (destStr s) "\^@") (MAP Str ls))) ++ [CHR 0]`,
+  Induct \\ rw[] \\ Cases_on `ls` \\ rw[FRONT_APPEND] 
+  \\ simp_tac std_ss [GSYM APPEND_ASSOC, GSYM CONS_APPEND, FRONT_APPEND] \\ rw[]
+  \\ rw[FRONT_DEF]
 );
 
-val map_app_count_thm = Q.prove(
-  `!ls a. ~(EXISTS (\x. x = a) (FLAT ls)) ==> 
-    LIST_ELEM_COUNT a (FLAT(MAP (\y. y ++ [a]) ls)) = LENGTH ls`,
-    Induct \\ rw[LIST_ELEM_COUNT_DEF, FILTER_APPEND_DISTRIB]
-    \\ fs[o_DEF, GSYM FILTER_EQ_NIL, LIST_ELEM_COUNT_DEF] 
+val CHR_w2n_n2w_ORD = Q.prove(
+  `(CHR o w2n o (n2w:num->word8) o ORD) = I`,
+  rw[o_DEF, ORD_BOUND, CHR_ORD, FUN_EQ_THM]
 );
 
-val map_app_count_Str = Q.prove(
-  `!ls. ~(EXISTS (\x. x = #"\^@") (FLAT ls)) ==> 
-    LIST_ELEM_COUNT #"\^@" (CONCAT(MAP (\s. STRCAT (destStr s) "\^@") (MAP Str ls) )) = LENGTH ls`,
-    Induct \\ rw[LIST_ELEM_COUNT_DEF, FILTER_APPEND_DISTRIB]
-    \\ fs[o_DEF, GSYM FILTER_EQ_NIL, LIST_ELEM_COUNT_DEF] 
+val validArg_def = Define`
+    validArg l <=>  (l <> []) /\ EVERY (\x. x <> #"\^@") l /\ LENGTH l < 256`;
+
+val TOKENS_MAP_inv = Q.store_thm ("TOKENS_MAP_inv",
+`!ls P l1. (P = (\x. x = #"\^@")) /\ EVERY validArg ls /\ l1 = (FLAT (MAP (\s. s ++ "\^@") ls)) ==>
+ (TOKENS P l1 = ls)`,
+  gen_tac \\ Induct_on `ls`
+  \\ rw[TOKENS_def] \\ Cases_on `h` \\ fs[validArg_def]
+  \\ rw[TOKENS_def]
+  \\ pairarg_tac \\ fs[NULL_EQ]
+  \\ rw[]
+  >-(imp_res_tac SPLITP_NIL_IMP \\ fs[validArg_def])
+  \\ (Cases_on `r`
+    >-(imp_res_tac SPLITP_NIL_SND_EVERY \\ fs[])
+    \\ fs[SPLITP] \\ rfs[]
+    \\ full_simp_tac std_ss [GSYM APPEND_ASSOC] 
+    \\ fs[SPLITP_APPEND] 
+    \\ Cases_on `EXISTS (\x. x = #"\^@") t` >- (full_simp_tac std_ss [EVERY_NOT_EXISTS])
+    \\ full_simp_tac std_ss [] \\ fs[SPLITP])
+  \\ rw[TOKENS_START]
+);
+
+val TOKENS_FRONT_MAP = Q.prove(
+  `!ls. ls <> [] ==> TOKENS (\x. x = #"\^@") (FRONT (FLAT (MAP (\x. x ++ "\^@") ls))) = TOKENS (\x. x = #"\^@") (FLAT (MAP (\x. x ++ "\^@") ls))`,
+  rw[map_app_last_thm, TOKENS_END, FRONT_APPEND]
 );
 
 
-(* Need to include that cl has no null characters 
+val TOKENS_FRONT_MAP_inv = Q.store_thm ("TOKENS_MAP_inv",
+  `!ls P. (P = (\x. x = #"\^@")) /\ EVERY validArg ls /\ ls <> []==> TOKENS P (FRONT(FLAT (MAP (\s. s ++ "\^@") ls))) = ls`,
+  rw[TOKENS_FRONT_MAP, TOKENS_MAP_inv] 
+);
+
+val hd_v_thm = fetch "mllistProg" "hd_v_thm";
+val mlstring_hd_v_thm = save_thm("mlstring_hd_v_thm",
+  hd_v_thm |> INST_TYPE [alpha |-> mlstringSyntax.mlstring_ty])
+
+(* replace TOKENS_EMPTY in misc with this *)
+val TOKENS_NIL = Q.store_thm("TOKENS_NIL",
+  `!ls. (TOKENS f ls = []) <=> EVERY f ls`,
+  Induct \\ rw[TOKENS_def]  \\ pairarg_tac  \\ fs[NULL_EQ, SPLITP] 
+  \\ every_case_tac \\ fs[] \\ rw[]);
+
+val MEM_REPLICATE_IMP = Q.store_thm("MEM_REPLICATE_IMP",
+  `MEM x (REPLICATE n y) ==> x = y`,
+  Induct_on`n` \\ rw[REPLICATE] \\ fs[]);
+
+val commandLine_cline_spec = Q.store_thm("commandLine_cline_spec",
+  `UNIT_TYPE u uv /\ cl <> [] /\ EVERY validArg cl /\ l = MAP ((n2w:num -> word8) o ORD) (FLAT (MAP (\s. (destStr s) ++ [CHR 0]) (MAP Str cl)))
+    /\ LENGTH l < 257 ==>
+    app (p:'ffi ffi_proj) ^(fetch_v "commandLine.cline" st) [uv]
+    (COMMANDLINE cl)
+    (POSTv clinev. & LIST_TYPE STRING_TYPE (MAP implode  cl) clinev * COMMANDLINE cl)`,
+    xcf "commandLine.cline" st
+    \\ xlet `POSTv cs. W8ARRAY cs (REPLICATE 256 (n2w 0)) * COMMANDLINE cl` 
+      >-(xapp \\ xsimpl)
+    \\ fs [COMMANDLINE_def] 
+    \\ xlet `POSTv zv. W8ARRAY cs (l ++ DROP (LENGTH l) (REPLICATE 256 (n2w 0))) * & (UNIT_TYPE () zv) * COMMANDLINE cl`
+    >-(xffi \\ fs [COMMANDLINE_def]
+      \\ map_every qexists_tac [`REPLICATE 256 (n2w 0)`,  `emp`, `l ++ DROP (LENGTH l) (REPLICATE 256 (n2w 0))`, `List (MAP Str cl)`, `List (MAP Str cl)`, `commandLine_fun`, `["getArgs"]`]
+      \\ xsimpl \\ fs[commandLine_fun_def]  \\ simp[EVERY_MAP, LENGTH_REPLICATE] \\ rw[] \\ fs[])
+    \\ xapp \\ xsimpl \\ gen_tac \\ strip_tac 
+    \\  reverse (conj_tac)  >-(fs[COMMANDLINE_def] \\ xsimpl)
+    \\ pop_assum mp_tac  
+    \\ simp[MAP_MAP_o, CHR_w2n_n2w_ORD] 
+    \\ simp[GSYM MAP_MAP_o]
+    \\ drule map_app_last_Str
+    \\ disch_then SUBST_ALL_TAC
+    \\ simp[mlstringTheory.implode_STRCAT, GSYM mlstringTheory.str_def, mlstringTheory.strcat_assoc, mlstringTheory.tokens_append]
+    \\ qmatch_abbrev_tac`_ _ l1 _ ==> _ _ l2 _`
+    \\ `l1 = l2` suffices_by rw[]
+    \\ simp[Abbr`l1`,Abbr`l2`] 
+    \\ Q.ISPEC_THEN`explode`match_mp_tac INJ_MAP_EQ 
+    \\ simp[MAP_MAP_o, INJ_DEF, mlstringTheory.explode_11, o_DEF, mlstringTheory.explode_implode, mlstringTheory.TOKENS_eq_tokens_sym]
+    \\ qmatch_abbrev_tac`TOKENS P l1 ++ TOKENS P l2 = _`
+    \\ `TOKENS P l2 = []`
+    by (
+      simp[TOKENS_NIL,Abbr`l2`,EVERY_MAP,EVERY_MEM]
+      \\ rw[] \\ imp_res_tac MEM_DROP_IMP
+      \\ imp_res_tac MEM_REPLICATE_IMP \\ fs[Abbr`P`] )
+    \\ simp[Abbr`l1`,Abbr`P`]
+    \\ match_mp_tac TOKENS_FRONT_MAP_inv
+    \\ simp[]
+);
+
 val commandLine_name_spec = Q.store_thm("commandLine_name_spec",
-  `UNIT_TYPE u uv /\ (cl <> []) ==>
+  `UNIT_TYPE u uv /\ (cl <> []) /\ (EVERY validArg cl) /\
+    LENGTH (MAP ((n2w:num -> word8) o ORD) (FLAT (MAP (\s. (destStr s) ++ [CHR 0]) (MAP Str cl)))) < 257 ==>
+    app (p:'ffi ffi_proj) ^(fetch_v "commandLine.name" st) [uv]
+    (COMMANDLINE cl)
+    (POSTv namev. & STRING_TYPE (implode (HD cl)) namev * COMMANDLINE cl)`,
+    xcf "commandLine.name" st
+    \\ xlet `POSTv vz. & UNIT_TYPE () vz * COMMANDLINE cl`
+    >-(xcon \\ xsimpl)
+    \\ xlet `POSTv cs. & LIST_TYPE STRING_TYPE (MAP implode cl) cs * COMMANDLINE cl` 
+    >-(xapp \\ rw[])
+    \\ xapp \\ xsimpl \\ instantiate \\ Cases_on `cl` \\ rw[]
+);
+
+val tl_v_thm = fetch "mllistProg" "tl_v_thm";
+val mlstring_tl_v_thm = save_thm("mlstring_tl_v_thm",
+  tl_v_thm |> INST_TYPE [alpha |-> mlstringSyntax.mlstring_ty])
+
+
+val commandLine_arguments_spec = Q.store_thm("commandLine_arguments_spec",
+  `UNIT_TYPE u uv /\ (cl <> []) /\ (EVERY validArg cl) /\
+    LENGTH (MAP ((n2w:num -> word8) o ORD) (FLAT (MAP (\s. (destStr s) ++ [CHR 0]) (MAP Str cl)))) < 257 ==>
+    app (p:'ffi ffi_proj) ^(fetch_v "commandLine.arguments" st) [uv]
+    (COMMANDLINE cl)
+    (POSTv namev. & LIST_TYPE STRING_TYPE (TL (MAP implode cl)) namev * COMMANDLINE cl)`,
+    xcf "commandLine.arguments" st
+    \\ xlet `POSTv vz. & UNIT_TYPE () vz * COMMANDLINE cl`
+    >-(xcon \\ xsimpl)
+    \\ xlet `POSTv cs. & LIST_TYPE STRING_TYPE (MAP implode cl) cs * COMMANDLINE cl` 
+    >-(xapp \\ rw[])
+    \\ xapp \\ xsimpl \\ instantiate \\ Cases_on `cl` \\ rw[mllistTheory.tl_def]
+);
+
+
+(*
+val commandLine_name_spec = Q.store_thm("commandLine_name_spec",
+  `UNIT_TYPE u uv /\ (cl <> []) /\ (EVERY validArg cl)  ==>
     app (p:'ffi ffi_proj) ^(fetch_v "commandLine.name" st) [uv]
     (COMMANDLINE cl)
     (POSTv namev. & STRING_TYPE (implode (HD cl)) namev * COMMANDLINE cl)`,
     xcf "commandLine.name" st
     \\ fs [COMMANDLINE_def] \\ xpull
     \\ Cases_on `LENGTH (MAP ((n2w:num -> word8) o ORD) (FLAT (MAP (\s. (destStr s) ++ [CHR 0]) (MAP Str cl)))) < 257` 
+    >-(
+      qmatch_assum_abbrev_tac `LENGTH args < 257` 
+      \\ xlet `POSTv zv. IO (List (MAP Str cl)) commandLine_fun ["getArgs"] * 
+      W8ARRAY commandLine_state (args ++ DROP (LENGTH args) w) * & (UNIT_TYPE () zv)`
+      >-(xffi \\ fs [EVAL ``commandLine_state``, COMMANDLINE_def]
+        \\ map_every qexists_tac [`w`,  `emp`, `args ++ DROP (LENGTH args) w`, `List (MAP Str cl)`, `List (MAP Str cl)`, `commandLine_fun`, `["getArgs"]`]
+        \\ xsimpl \\ fs[commandLine_fun_def, Abbr `args`] \\ simp[EVERY_MAP])
+      \\ xlet `POSTv strlv. SEP_EXISTS ss. &LIST_TYPE STRING_TYPE ss strlv * & (TAKE (LENGTH cl) ss = MAP implode cl) * IO (List (MAP Str cl)) commandLine_fun ["getArgs"] * 
+          W8ARRAY commandLine_state (args ++ DROP (LENGTH args) w) `  
       >-(
-        qmatch_assum_abbrev_tac `LENGTH args < 257` 
-        \\ xlet `POSTv zv. IO (List (MAP Str cl)) commandLine_fun ["getArgs"] * 
-        W8ARRAY commandLine_state (args ++ DROP (LENGTH args) w) * & (UNIT_TYPE () zv)`
-        >-(xffi \\ fs [EVAL ``commandLine_state``, COMMANDLINE_def]
-          \\ map_every qexists_tac [`w`,  `emp`, `args ++ DROP (LENGTH args) w`, `List (MAP Str cl)`, `List (MAP Str cl)`, `commandLine_fun`, `["getArgs"]`]
-          \\ xsimpl \\ fs[commandLine_fun_def, Abbr `args`] \\ simp[EVERY_MAP])
+        xapp \\ xsimpl 
+        \\ qexists_tac `IO (List (MAP Str cl)) commandLine_fun ["getArgs"]` 
+        \\ qexists_tac `args ++ DROP (LENGTH args) w`
+        \\ fs[EVAL ``commandLine_state``] \\ xsimpl
+        \\ rpt strip_tac \\ instantiate 
+        \\ fs[Abbr `args`]
+        \\ qmatch_abbrev_tac`TAKE (LENGTH cl) ls = _`
+        \\ `IS_PREFIX ls (MAP implode cl)` suffices_by
+        ( rw[IS_PREFIX_APPEND,TAKE_APPEND1]
+        \\ rw[TAKE_APPEND1,TAKE_LENGTH_ID_rwt] )
+        \\ simp[Abbr`ls`]
+        \\ simp[IS_PREFIX_APPEND]
+        \\ simp[MAP_MAP_o, CHR_w2n_n2w_ORD] 
+        \\ simp[GSYM MAP_MAP_o]
+        \\ drule map_app_last_Str
+        \\ disch_then SUBST_ALL_TAC
+        \\ rw[mlstringTheory.implode_STRCAT, GSYM mlstringTheory.str_def, mlstringTheory.strcat_assoc, mlstringTheory.tokens_append]
+        \\ qexists_tac `tokens (\x. x = #"\^@") (implode (MAP CHR (MAP w2n (DROP (STRLEN (FRONT (FLAT (MAP (\s. STRCAT (destStr s) "\^@") (MAP Str cl)))) + 1) w))))`
+        \\ rw[] 
+        (*now tokens is isolated*)
+        \\ Q.ISPEC_THEN`explode`match_mp_tac INJ_MAP_EQ 
+        \\ simp[MAP_MAP_o, INJ_DEF, mlstringTheory.explode_11, o_DEF, mlstringTheory.explode_implode, mlstringTheory.TOKENS_eq_tokens_sym]
+        \\ rw[TOKENS_FRONT_MAP_inv])
+      \\ xapp \\ xsimpl \\ fs [Abbr `args`] 
+      \\ instantiate
+      \\ `MAP implode cl <> []` by fs[MAP_EQ_NIL]
+      \\ `TAKE (LENGTH cl) ss <> []` by metis_tac[]
+      \\ fs[TAKE_EQ_NIL]
+      \\ Cases_on `cl` \\ fs[]
+      \\ Cases_on `ss` \\ fs[]
+    )
+    (*the commandline is too long here*)
+    \\ qmatch_assum_abbrev_tac `¬(LENGTH args < 257)`
+    \\ xlet `POSTv zv. IO (List (MAP Str cl)) commandLine_fun ["getArgs"] * 
+      W8ARRAY commandLine_state (TAKE 256 args) * & (UNIT_TYPE () zv)`
+    >-(xffi \\ fs [EVAL ``commandLine_state``, COMMANDLINE_def]
+      \\ map_every qexists_tac [`w`,  `emp`, `TAKE 256 args`, `List (MAP Str cl)`, `List (MAP Str cl)`, `commandLine_fun`, `["getArgs"]`]
+      \\ xsimpl \\ fs[commandLine_fun_def, Abbr `args`] \\ simp[EVERY_MAP, MAP_TAKE] \\ xsimpl)
+    \\ xlet `POSTv strlv. & LIST_TYPE STRING_TYPE (tokens (\x. x = #"\^@") (implode (TAKE 256 (FLAT (MAP (\l. l ++ "\^@") cl))))) strlv
+        * IO (List (MAP Str cl)) commandLine_fun ["getArgs"] * W8ARRAY commandLine_state (TAKE 256 args)`
+    >-(xapp \\ xsimpl
+      \\ qexists_tac `IO (List (MAP Str cl)) commandLine_fun ["getArgs"]` 
+      \\ qexists_tac `TAKE 256 args`
+      \\ fs[EVAL ``commandLine_state``] \\ xsimpl
+      \\ rpt strip_tac \\ fs[Abbr `args`]
+      \\ fs[MAP_MAP_o, CHR_w2n_n2w_ORD, MAP_TAKE]
+      \\ fs[GSYM MAP_MAP_o]
+      \\ fs[destStr_str] )
+    \\ xapp \\ xsimpl \\ instantiate
+    \\ fs[LENGTH_NIL, LENGTH_TAKE_EQ, validArg_def, EVERY_MEM]
+    \\ rw[mlstringTheory.TOKENS_eq_tokens_sym, mlstringTheory.explode_implode]
+    >-(
+      CCONTR_TAC \\ fs[]
+      \\ imp_res_tac TOKENS_EMPTY
+      \\ `MAP (\x. STRCAT x "\^@") cl <> []` by fs[MAP_EQ_NIL]
+      \\ `CONCAT (MAP (\x. STRCAT x "\^@") cl) <> []` by fs[FLAT_EQ_NIL] >-(Cases_on `cl` \\ rw[])
+      \\ fs[LENGTH_NIL, LENGTH_TAKE_EQ]
+      \\ Cases_on `cl` \\ fs[]
+      \\ Cases_on `h` >-(last_x_assum (qspecl_then [`""`] mp_tac) \\ rw[])
+      \\ first_x_assum (qspecl_then [`h'`] mp_tac) \\ rw[]
+      \\ metis_tac[MEM])
+    \\ Cases_on `cl` \\ fs[Once TAKE_APPEND]
+    \\ first_x_assum (qspecl_then [`h`] mp_tac) \\ rw[]
+    \\ fs[TAKE_LENGTH_TOO_LONG]
+    \\ full_simp_tac std_ss [GSYM APPEND_ASSOC, GSYM CONS_APPEND, TOKENS_APPEND]
+    \\ fs[MAP_APPEND]
+    \\ `validArg h` by fs [validArg_def, EVERY_MEM]
+    \\ fs[validArg_TOKENS]
+);    
 
-        (* \\ xlet `POSTv strlv. &LIST_TYPE STRING_TYPE (MAP implode cl ++ [implode (MAP (CHR o w2n) (DROP (LENGTH args) w))]) strlv` *) 
-        \\ xlet `POSTv strlv. SEP_EXISTS ss. &LIST_TYPE STRING_TYPE ss strlv * & (TAKE (LENGTH cl) ss = MAP implode cl)`  
-        >-(
-          xapp \\ xsimpl 
-          \\ qexists_tac `IO (List (MAP Str cl)) commandLine_fun ["getArgs"]` 
-          \\ qexists_tac `args ++ DROP (LENGTH args) w`
-          \\ fs[EVAL ``commandLine_state``] \\ xsimpl
-          \\ rpt strip_tac \\ instantiate 
-          \\ fs[Abbr `args`]
-          \\ rw[map_app_last_Str]
-          \\ rfs[mlstringTheory.tokens_def, mlstringTheory.tokens_aux_def]
-          \\ cheat
-          )
-        \\ xapp \\ xsimpl \\ qexists_tac `ss`
-          
+val validArg_TOKENS = Q.prove(
+  `!l. validArg l ==> TOKENS (\x. x = #"\^@") l = [l]`,
+    Induct \\ rw[validArg_def, TOKENS_def]
+    \\ pairarg_tac \\ fs[NULL_EQ] \\ rw[]
+    >-(Cases_on `r` \\ imp_res_tac SPLITP_JOIN \\ fs[]
+      \\ imp_res_tac SPLITP_NIL_IMP \\ fs[])
+    >-(Cases_on `r` >-(imp_res_tac SPLITP_NIL_SND_EVERY \\ fs[])
+      \\ imp_res_tac SPLITP_CONS_IMP \\ fs[] \\ full_simp_tac std_ss [EVERY_NOT_EXISTS])
+    \\ Cases_on `r` >-(rw[TOKENS_def]) 
+      \\ imp_res_tac SPLITP_CONS_IMP \\ fs[] \\ full_simp_tac std_ss [EVERY_NOT_EXISTS]
+);
+ 
 
 
-          \\ qexists_tac `IO (Str cl) commandLine_fun ["getArgs"]` \\ qexists_tac `MAP (n2w o ORD) cl ++ DROP (LENGTH cl) w` 
-          \\ rw [EVAL ``commandLine_state``] \\ xsimpl)
-        \\ instantiate
-
-mlstringTheory.tokens_filter
-
-
-DB.match[]`` ``
-DB.match[]``MAP (MAP _) _`` 
-DB.match[]``MAP _ (FLAT _) = FLAT (MAP _ _)``
-  \\ xapp_prepare_goal
-        val (asl, w) = top_goal()
-        val (ffi_ty, f) = goal_app_infos w
-        xspec ffi_ty f xapp_xapply_no_simpl
-        xspec_in_db f
-
-        is_arrow_spec_for f (concl mllistProgTheory.hd_v_thm)
-        val tm = ()
-
-DB.find"n2w"
-
-val hd1_v_thm = save_thm("hd1_v_thm",
-  mllistProgTheory.hd_v_thm |> |> UNDISCH_ALL)
-
-
-        goal_app_infos 
-
-
-        xapp_xapply_no_simpl
-        xspec ffi_ty f 
-        \\ xapp_prepare_goal
-        val (asl,w) = top_goal()
-    spec_kind_for (#2 (goal_app_infos w))
-    xapp_spec
-        goal_app_infos
-        \\ tmtac
-       
-fetch_v "List.hd" st
-
-
-        \\ xsimpl
-        \\ `MEM "getArgs" ["getArgs"]` by EVAL_TAC \\ fs[commandLine_fun_def] \\ instantiate
-      )
-    \\ IO (Str cl) commandLine_fun ["getArgs"] * W8ARRAY commandLine_state [w]`
-    \\ xlet `POSTv zv. W8ARRAY 
-DB.find "REPLICATE"
-val commandLine_arguments_spec = Q.store_thm("commandLine_arguments_spec",
-    `UNIT_TYPE u uv ==>
-     app (p:'ffi ffi_proj) ^(fetch_v "commandLine.name" (hi())) [uv]
-    (COMMANDLINE cl)
-    (POSTv namev. & STRING_TYPE (tl (tokens (\x. x = (CHR 0)) cl)) namev * COMMANDLINE cl)`
-    
 *)
-(*AIM: to be able to define echo using the arguments function so that
+
+(*
+AIM: to be able to define echo using the arguments function so that
   `!cl. (*some specification about length of cl being less than 256*) ==>
   app (p:'ffi ffi_proj) echo_v [uv] (COMMANDLINE cl * STDOUT out)
   (POSTv u. COMMANDLINE cl * STDOUT (out ++ (CONCAT (MAP implode (arguments cl)))))`
 
   is true *)
 *)
-val _ = export_theory()
+val _ = export_theory();
 
